Changes for second isomorphism PR

theory/ua_second_isomorphism.v
@@ -1,50 +1,48 @@
-(*
-
-(** This files proves the second isomorphism theorem in two ways.
-    The first way is direct and the other way uses the first
-    isomorphism theorem. From a software engineering perspective it
-    may make sense to split the results in this file to other files. *)
+(** The second isomorphism theorem [isomorphic_second_isomorphism]. *)
 
 Require Import
   HoTT.Types.Sigma
   HoTT.Types.Universe
+  HoTT.HSet
   HoTT.HIT.quotient
-  HoTTClasses.theory.ua_homomorphism
+  HoTT.Classes.interfaces.canonical_names
+  HoTTClasses.theory.ua_isomorphic
   HoTTClasses.theory.ua_subalgebra
-  HoTTClasses.theory.ua_quotient_algebra
-  HoTTClasses.theory.ua_first_isomorphism.
+  HoTTClasses.theory.ua_quotient_algebra.
 
 Import
   algebra_notations
   quotient_algebra_notations
-  subalgebra_notations.
+  subalgebra_notations
+  isomorphic_notations.
 
-Local Notation i := (hom_inclusion_subalgebra _).
+Local Notation i := (hom_inc_subalgebra _ _).
+
+(** This section defines [cong_trace] and proves that it is a
+    congruence, the restriction of a congruence to a subalgebra. *)
 
 Section cong_trace.
   Context
-    {σ : Signature}
-    {A : Algebra σ}
-    (P : SubalgebraPredicate A)
-    (Φ : Congruence A).
+    {σ : Signature} {A : Algebra σ}
+    (P : ∀ s, A s → Type) `{!IsSubalgebraPredicate A P}
+    (Φ : ∀ s, relation (A s)) `{!IsCongruence A Φ}.
 
-  Definition relation_trace (s : Sort σ) (x : (A&P) s) (y : (A&P) s)
-    : Type
+  Definition cong_trace (s : Sort σ) (x : (A&P) s) (y : (A&P) s)
     := Φ s (i s x) (i s y).
 
-  Global Instance equivalence_trace_congruence (s : Sort σ)
-    : Equivalence (relation_trace s).
+  Global Instance equiv_rel_trace_congruence (s : Sort σ)
+    : EquivRel (cong_trace s).
   Proof.
-    unfold relation_trace.
+    unfold cong_trace.
     constructor.
     - intros [y Y]. reflexivity.
     - intros [y1 Y1] [y2 Y2] S. by symmetry.
     - intros [y1 Y1] [y2 Y2] [y3 Y3] S T. by transitivity y2.
-  Defined.
+  Qed.
 
   Lemma for_all_2_family_prod_trace_congruence {w : SymbolType σ}
     (a b : FamilyProd (A&P) (dom_symboltype w))
-    (R : for_all_2_family_prod (A&P) (A&P) relation_trace a b)
+    (R : for_all_2_family_prod (A&P) (A&P) cong_trace a b)
     : for_all_2_family_prod A A Φ
         (map_family_prod i a) (map_family_prod i b).
   Proof with try assumption.
@@ -54,92 +52,101 @@ Section cong_trace.
     apply IHw...
   Qed.
 
-  Definition has_congruence_property_trace
-    : HasCongruenceProperty (A&P) relation_trace.
+  Global Instance ops_compatible_trace_trace
+    : OpsCompatible (A&P) cong_trace.
   Proof.
     intros u a b R.
     refine (transport (λ X, Φ _ X _)
-              (path_ap_operation_inclusion_subalgebra P u a) _).
+              (path_homomorphism_ap_operation i u a)^ _).
     refine (transport (λ X, Φ _ _ X)
-              (path_ap_operation_inclusion_subalgebra P u b) _).
-    apply (property_congruence Φ).
+              (path_homomorphism_ap_operation i u b)^ _).
+    apply (ops_compatible_cong A Φ).
     exact (for_all_2_family_prod_trace_congruence a b R).
   Qed.
 
-  Definition cong_trace : Congruence (A&P)
-    := BuildCongruence relation_trace has_congruence_property_trace.
-
+  Global Instance is_congruence_trace : IsCongruence (A&P) cong_trace.
+  Proof.
+    apply (@BuildIsCongruence _ (A&P) cong_trace);
+      [intros; apply (is_mere_relation_cong A Φ) | exact _ ..].
+  Qed.
 End cong_trace.
 
-Section in_subquotient.
-  Context
-    `{Univalence}
-    {σ : Signature}
-    {A : Algebra σ}
-    (P : SubalgebraPredicate A)
-    (Φ : Congruence A).
+(** The following section defines the [is_subalgebra_class] subalgebra
+    predicate, which induces a subalgebra of [A/Φ]. *)
 
-  Definition def_in_subquotient (s : Sort σ) (x : (A/Φ) s) : hProp
+Section is_subalgebra_class.
+  Context `{Univalence}
+    {σ : Signature} {A : Algebra σ}
+    (P : ∀ s, A s → Type) `{!IsSubalgebraPredicate A P}
+    (Φ : ∀ s, relation (A s)) `{!IsCongruence A Φ}.
+
+  Definition is_subalgebra_class (s : Sort σ) (x : (A/Φ) s) : hProp
     := hexists (λ (y : (A&P) s), in_class (Φ s) x (i s y)).
 
-  Lemma op_closed_subalgebra_in_subquotient {w : SymbolType σ}
+  Lemma op_closed_subalgebra_is_subalgebra_class {w : SymbolType σ}
     (γ : Operation (A/Φ) w)
     (α : Operation A w)
-    (Q : QuotientOpProperty A Φ α γ)
+    (Q : ComputeOpQuotient A Φ α γ)
     (C : ClosedUnderOp A P α)
-    : ClosedUnderOp (A/Φ) def_in_subquotient γ.
+    : ClosedUnderOp (A/Φ) is_subalgebra_class γ.
   Proof.
     induction w.
-    - specialize (Q tt). cbn in Q.
-      apply tr.
+    - specialize (Q tt). apply tr.
       exists (α; C).
-      unfold i, def_inclusion_subalgebra.
-      rewrite Q.
-      exact (Equivalence_Reflexive α).
+      cbn in Q. destruct Q^.
+      exact (EquivRel_Reflexive α).
     - refine (quotient_ind_prop (Φ t) _ _). intro x.
       refine (Trunc_rec _).
       intros [y R].
       apply (IHw (γ (class_of (Φ t) x)) (α (i t y))).
-      intro a.
-      rewrite (related_classes_eq (Φ t) R).
-      apply (Q (i t y,a)).
-      apply C.
-      exact y.2.
+      + intro a.
+        destruct (related_classes_eq (Φ t) R)^.
+        apply (Q (i t y,a)).
+      + apply C. exact y.2.
   Qed.
 
-  Definition is_closed_under_ops_in_subquotient
-    : IsClosedUnderOps (A/Φ) def_in_subquotient.
+  Definition is_closed_under_ops_is_subalgebra_class
+    : IsClosedUnderOps (A/Φ) is_subalgebra_class.
   Proof.
     intro u.
-    eapply op_closed_subalgebra_in_subquotient.
-    apply quotient_op_property.
-    apply is_closed_under_ops_subalgebra_predicate.
+    eapply op_closed_subalgebra_is_subalgebra_class.
+    - apply compute_op_quotient.
+    - apply is_closed_under_ops_subalgebra_predicate. exact _.
   Qed.
 
-  Definition in_subquotient : SubalgebraPredicate (A/Φ)
-    := BuildSubalgebraPredicate
-        def_in_subquotient
-        is_closed_under_ops_in_subquotient.
+  Global Instance is_subalgebra_predicate_is_subalgebra_class
+    : IsSubalgebraPredicate (A/Φ) is_subalgebra_class.
+  Proof.
+    apply BuildIsSubalgebraPredicate.
+    apply is_closed_under_ops_is_subalgebra_class.
+  Qed.
+End is_subalgebra_class.
 
-End in_subquotient.
+(** The next section proves the second isomorphism theorem,
+
+    <<
+      (A&P) / (cong_trace P Φ) ≅ (A/Φ) & (is_subalgebra_class P Φ).
+    >>
+*)
+
+(* There is an alternative proof using the first isomorphism theorem,
+   but the direct proof below seems simpler in HoTT. *)
 
 Section second_isomorphism.
-  Context
-    `{Univalence}
-    {σ : Signature}
-    {A : Algebra σ}
-    (P : SubalgebraPredicate A)
-    (Φ : Congruence A).
+  Context `{Univalence}
+    {σ : Signature} (A : Algebra σ)
+    (P : ∀ s, A s → Type) `{!IsSubalgebraPredicate A P}
+    (Φ : ∀ s, relation (A s)) `{!IsCongruence A Φ}.
 
   Local Notation Ψ := (cong_trace P Φ).
 
-  Local Notation Q := (in_subquotient P Φ).
+  Local Notation Q := (is_subalgebra_class P Φ).
 
   Definition def_second_isomorphism (s : Sort σ)
     : ((A&P) / Ψ) s → ((A/Φ) & Q) s
     := quotient_rec (Ψ s)
         (λ (x : (A&P) s),
-         (class_of (Φ s) (i s x); tr (x; Equivalence_Reflexive x)))
+         (class_of (Φ s) (i s x); tr (x; EquivRel_Reflexive x)))
         (λ (x y : (A&P) s) (T : Ψ s x y),
          path_sigma_hprop (class_of (Φ s) (i s x); _)
            (class_of (Φ s) (i s y); _) (related_classes_eq (Φ s) T)).
@@ -147,14 +154,14 @@ Section second_isomorphism.
   Lemma oppreserving_second_isomorphism {w : SymbolType σ}
     (α : Operation A w) (γ : Operation (A/Φ) w)
     (ζ : Operation ((A&P) / Ψ) w) (CA : ClosedUnderOp (A/Φ) Q γ)
-    (CB : ClosedUnderOp A P α) (QA : QuotientOpProperty A Φ α γ)
-    (QB : QuotientOpProperty (A&P) Ψ (op_subalgebra P α CB) ζ)
-    : OpPreserving def_second_isomorphism ζ (op_subalgebra Q γ CA).
+    (CB : ClosedUnderOp A P α) (QA : ComputeOpQuotient A Φ α γ)
+    (QB : ComputeOpQuotient (A&P) Ψ (op_subalgebra A P α CB) ζ)
+    : OpPreserving def_second_isomorphism ζ (op_subalgebra (A/Φ) Q γ CA).
   Proof.
-    unfold QuotientOpProperty in *.
+    unfold ComputeOpQuotient in *.
     induction w; cbn in *.
     - apply path_sigma_hprop.
-      rewrite (QB tt), (QA tt).
+      cbn. destruct (QB tt)^, (QA tt)^.
       by apply related_classes_eq.
     - refine (quotient_ind_prop (Ψ t) _ _). intro x.
       apply (IHw (α (i t x)) (γ (class_of (Φ t) (i t x)))
@@ -163,25 +170,25 @@ Section second_isomorphism.
               (CB (i t x) x.2)).
       + intro a. exact (QA (i t x, a)).
       + intro a. exact (QB (x, a)).
-  Qed.
+  Defined.
 
-  Definition is_homomorphism_second_isomorphism
+  Global Instance is_homomorphism_second_isomorphism
     : IsHomomorphism def_second_isomorphism.
   Proof.
     intro u.
     eapply oppreserving_second_isomorphism.
-    apply (quotient_op_property A).
-    apply (quotient_op_property (A&P)).
-  Qed.
+    - apply (compute_op_quotient A).
+    - apply (compute_op_quotient (A&P)).
+  Defined.
 
   Definition hom_second_isomorphism
     : Homomorphism ((A&P) / Ψ) ((A/Φ) & Q)
-    := BuildHomomorphism
-        def_second_isomorphism is_homomorphism_second_isomorphism.
+    := BuildHomomorphism def_second_isomorphism.
 
-  Global Instance injection_second_isomorphism (s : Sort σ)
-    : Injective (hom_second_isomorphism s).
+  Global Instance embedding_second_isomorphism (s : Sort σ)
+    : IsEmbedding (hom_second_isomorphism s).
   Proof.
+    apply isembedding_isinj_hset.
     refine (quotient_ind_prop (Ψ s) _ _). intro x.
     refine (quotient_ind_prop (Ψ s) _ _). intros y p.
     apply related_classes_eq.
@@ -196,8 +203,7 @@ Section second_isomorphism.
     generalize dependent S.
     generalize dependent y.
     refine (quotient_ind_prop (Φ s) _ _). intros y S.
-    refine (Trunc_rec _ S). intros [y' S'].
-    apply tr.
+    refine (Trunc_rec _ S). intros [y' S']. apply tr.
     exists (class_of _ y').
     apply path_sigma_hprop.
     by apply related_classes_eq.
@@ -206,124 +212,18 @@ Section second_isomorphism.
   Theorem is_isomorphism_second_isomorphism
     : IsIsomorphism hom_second_isomorphism.
   Proof.
-    constructor; exact _.
+    intro s. apply isequiv_surj_emb; exact _.
   Qed.
 
   Global Existing Instance is_isomorphism_second_isomorphism.
 
-  Corollary path_second_isomorphism : (A&P) / Ψ = (A/Φ) & Q.
+  Theorem isomorphic_second_isomorphism : (A&P) / Ψ ≅ (A/Φ) & Q.
   Proof.
-    exact (path_isomorphism hom_second_isomorphism).
+    exact (BuildIsomorphic def_second_isomorphism).
+  Defined.
+
+  Corollary id_second_isomorphism : (A&P) / Ψ = (A/Φ) & Q.
+  Proof.
+    exact (id_isomorphic isomorphic_second_isomorphism).
   Defined.
 End second_isomorphism.
-
-Section second_isomorphism'.
-  Context
-    `{Univalence}
-    {σ : Signature}
-    (A : Algebra σ)
-    (P : SubalgebraPredicate A)
-    (Φ : Congruence A).
-
-  Local Notation Ψ := (cong_trace P Φ).
-
-  Local Notation Q := (in_subquotient P Φ).
-
-  Definition def_second_surjection (s : Sort σ) (x : (A&P) s)
-    : ((A/Φ) & Q) s
-    := (class_of (Φ s) (i s x); tr (x; Equivalence_Reflexive x)).
-
-  Lemma oppreserving_second_surjection {w : SymbolType σ}
-    (α : Operation A w)
-    (γ : Operation (A/Φ) w)
-    (Cγ : ClosedUnderOp (A/Φ) Q γ)
-    (Cα : ClosedUnderOp A P α)
-    (R : QuotientOpProperty A Φ α γ)
-    : OpPreserving def_second_surjection
-        (op_subalgebra P α Cα) (op_subalgebra Q γ Cγ).
-  Proof.
-    unfold QuotientOpProperty in *.
-    induction w; cbn in *.
-    - apply path_sigma_hprop. symmetry. apply (R tt).
-    - intro x.
-      by specialize (IHw (α (i t x)) (γ (class_of (Φ t) (i t x)))
-       (Cγ (class_of (Φ t) (i t x)) (tr (x; Equivalence_Reflexive x)))
-       (Cα (i t x) x.2) (λ a, R (i t x, a))).
-  Qed.
-
-  Definition is_homomorphism_second_surjection
-    : IsHomomorphism def_second_surjection.
-  Proof.
-    intro u.
-    apply oppreserving_second_surjection.
-    apply (quotient_op_property A).
-  Qed.
-
-  Definition hom_second_surjection : Homomorphism (A&P) ((A/Φ) & Q)
-    := BuildHomomorphism
-        def_second_surjection is_homomorphism_second_surjection.
-
-  Global Instance surjection_second_surjection (s : Sort σ)
-    : IsSurjection (hom_second_surjection s).
-  Proof.
-    apply BuildIsSurjection.
-    intros [y Y].
-    generalize dependent Y.
-    generalize dependent y.
-    refine (quotient_ind_prop (Φ s) _ _).
-    intros y Y.
-    refine (Trunc_rec _ Y).
-    intros [y' Y'].
-    apply tr.
-    exists y'.
-    apply path_sigma_hprop.
-    by apply related_classes_eq.
-  Qed.
-
-  Lemma iff_second_surjection_cong_ker_trace (s : Sort σ) (x y : (A&P) s)
-    : cong_ker hom_second_surjection s x y ↔ Ψ s x y.
-  Proof.
-    split.
-    - intro K. apply (classes_eq_related (Φ s)). apply (K..1).
-    - intro T. apply path_sigma_hprop. by apply related_classes_eq.
-  Defined.
-
-  Lemma path_second_surjection_cong_ker_trace
-    : cong_ker hom_second_surjection = Ψ.
-  Proof.
-    apply path_congruence; try exact _.
-    apply iff_second_surjection_cong_ker_trace.
-  Defined.
-
-  Definition hom_second_isomorphism'
-    : Homomorphism ((A&P) / Ψ) ((A/Φ) & Q)
-    := transport (λ C, Homomorphism ((A&P) / C) (A/Φ & Q))
-          path_second_surjection_cong_ker_trace
-          (hom_surjective_first_isomorphism hom_second_surjection).
-
-  Theorem is_isomorphism_second_isomorphism'
-    : IsIsomorphism hom_second_isomorphism'.
-  Proof.
-    unfold hom_second_isomorphism'.
-    destruct path_second_surjection_cong_ker_trace.
-    exact _.
-  Qed.
-
-  Global Existing Instance is_isomorphism_second_isomorphism'.
-
-  Corollary path_second_isomorphism' : (A&P) / Ψ = (A/Φ) & Q.
-  Proof.
-    exact (path_isomorphism hom_second_isomorphism').
-  Defined.
-
-  Lemma path_hom_second_isomorphisms
-    : hom_second_isomorphism P Φ = hom_second_isomorphism'.
-  Proof.
-    apply path_homomorphism. intro s.
-    refine (quotient_ind_prop (Ψ s) _ _). intros [x E].
-    apply path_sigma_hprop.
-    unfold hom_second_isomorphism'.
-    by induction path_second_surjection_cong_ker_trace.
-  Defined.
-End second_isomorphism'.
-*)
