build.sh
@@ -1,0 +1,7 @@
+
+if [ -z "$1" ]; then
+  echo Missing HoTT dir >&2
+  exit 1
+fi
+
+make COQC="$1"/hoqc COQTOP="$1"/hoqtop COQDEP="$1"/hoqdep
